theories/tree_prop.v
@@ -13,19 +13,8 @@ Section RunP.
   (* EXPAND PROPERTIES                                                *)
   (********************************************************************)
 
-  Lemma is_ko_step u p fv A s1: is_ko A -> step u p fv  s1 A = (fv, Failed, A).
-  Proof.
-    elim: A s1 => //.
-    - move=> A HA s B HB s1 /= /andP[kA kB]; rewrite HA//.
-    - move=> s B HB s1/= kB; rewrite HB//.
-    - move=> A HA B0 B HB s1 /= kA; rewrite HA//.
-  Qed.
-
   Lemma failed_big_and t: failed (big_and t) = false.
   Proof. case: t => [|[]]//. Qed.
-
-  Lemma is_ko_big_and r: is_ko (big_and r) = false.
-  Proof. apply/contraFF/failed_big_and/r/is_ko_failed. Qed.
 
   (*SNIP: success_step*)
   Lemma success_step u p fv s A: success A -> step u p fv s A = (fv, Success, A).
@@ -33,8 +22,8 @@ Section RunP.
   Proof.
     elim: A s => //; try by do 2 eexists.
     + move=> A HA s1 B HB s /= sA; rewrite HA//.
-    + move=> s B HB/= _ sB; rewrite HB//.
-    + move=> A HA B0 B HB s /=/andP[sA sB]; rewrite HA//HB//.
+    + move=> s B HB/= _ /[!success_or_None] sB; rewrite HB//.
+    + move=> A HA B0 B HB s /=/[!success_and]/andP[sA sB]; rewrite HA//HB//.
   Qed.
 
   Ltac case_step_tag X A := let fv := fresh "_fv" in case X : step => [[fv []] A].
@@ -47,11 +36,12 @@ Section RunP.
     + by move=> /= ???? [? <-].
     + by move=> []//= ?????; case: backchain.
     + move=> A HA s B HB ?? s1 C/=.
-      by case_step_tag X B1 => //=-[??]; subst; rewrite !(HA _ _ _ _ X).
+      by case_step_tag X B1 => //=-[??]; subst; rewrite success_or_Some !(HA _ _ _ _ X).
     + move=> s B HB ?? s1 C/=.
-      by case_step_tag X B1 => //=-[??]; subst; rewrite !(HB _ _ _ _ X).
+      by case_step_tag X B1 => //=-[??]; subst; rewrite success_or_None !(HB _ _ _ _ X).
     + move=> A HA B0 B HB s1 ?? C /=.
       case_step_tag X A1 => //=; case_step_tag Y B1 => //= -[??]; subst.
+      rewrite success_and.
       have [[??]->] := HA _ _ _ _ X; subst.
       by rewrite !(HB _ _ _ _ Y).
   Qed.
@@ -65,10 +55,11 @@ Section RunP.
     + move=> ?? s1 B[<-]//.
     + by move=> []//= ?????; push.
     + move=> A HA s B HB ?? s1 C/=; push.
-      by case: ifP => dA /= [e + <-]{C}/=; do [case_step_tag S B1] in e * => //; subst; rewrite !(HA _ _ _ _ S).
+      by case: ifP => dA /= [e + <-]{C}/=; do [case_step_tag S B1] in e * => //; subst; rewrite failed_or_Some !(HA _ _ _ _ S).
     + move=> s B HB ?? s1 C/=; push.
-      by case: ifP => dA /= [e + <-]{C}/=; do [case_step_tag S B1] in e * => //; subst; rewrite !(HB _ _ _ _ S).
+      by case: ifP => dA /= [e + <-]{C}/=; do [case_step_tag S B1] in e * => //; subst; rewrite failed_or_None !(HB _ _ _ _ S).
     + move=> A HA B0 B HB ?? s1 C /=.
+      rewrite failed_and.
       case_step_tag X A1 => //=.
         by move=> -[??]; subst; rewrite !(HA _ _ _ _ X).
       case_step_tag Y B1 => //= -[??]; subst.
@@ -76,31 +67,19 @@ Section RunP.
       by rewrite !(HB _ _ _ _ Y) orbT.
   Qed.
 
-  Lemma is_ko_next_alt {A} b: is_ko A -> next_alt b A = None.
-  Proof.
-    elim: A b => //=.
-      by move=> A HA s1 B HB b /= /andP[kA kB]; rewrite HA//HB.
-      by move=> s1 B HB b /= kB; rewrite HB.
-    move=> A HA l B HB /= b kA.
-    by rewrite is_ko_success//HA//is_ko_failed.
-  Qed.
-
   Lemma next_alt_None_failed {A}: 
     next_alt false A = None -> failed A.
   Proof.
     elim: A => //=.
     - move=> A + s1 B +/=; do 2 case: next_alt => //.
-    - move=> s1 B +/=; case: next_alt => //.
+    - by move=> s1 B +/=; case: next_alt => //; rewrite failed_or_None.
     - move=> A + l B +.
+      rewrite failed_and.
       case sA: success.
         rewrite (success_failed sA)/=.
         by case: (next_alt _ B) => //=; auto.
       by case: ifP.
   Qed.
-
-  Lemma next_alt_cutr {A b}:
-    next_alt b (cutr A) = None.
-  Proof. apply: is_ko_next_alt is_ko_cutr. Qed.
 
   (* Lemma is_dead_next_alt {A} b: is_dead A -> next_alt b A = None.
   Proof. move=>/is_dead_is_ko/is_ko_next_alt//. Qed. *)
@@ -110,8 +89,8 @@ Section RunP.
   Proof.
     elim: A => //=.
     - move=> A HA s B HB sA; rewrite HA//is_ko_next_alt//.
-    - move=> s B HB sA; rewrite HB//is_ko_next_alt//.
-    - move=> A HA l B HB /andP[sA sB].
+    - move=> s B HB /[!success_or_None] sA; rewrite HB//.
+    - move=> A HA l B HB /[!success_and] /andP[sA sB].
       rewrite sA/= success_cut sA HA// HB//.
   Qed.
 
@@ -120,10 +99,10 @@ Section RunP.
   Proof.
     elim: A b => //=.
     - move=> A HA s B HB b fA; rewrite HA// is_ko_next_alt//.
-    - move=> s B HB b fA; rewrite HB// is_ko_next_alt//.
+    - move=> s B HB b /[!failed_or_None] fA; rewrite HB// is_ko_next_alt//.
     - move=> A HA l B HB b.
       case: ifP => sA//=.
-      rewrite failed_success_cut success_cut sA/=.
+      rewrite failed_and failed_success_cut success_cut sA/=.
       move=> fB.
       rewrite HB//=next_alt_cutl_success//.
   Qed.
@@ -152,8 +131,9 @@ Section RunP.
   Proof.
     elim: A s1; clear => //; try by move=> ? [] //.
     + move=> A HA s1 B HB s2/=fA; rewrite HA//.
-    + move=> s1 B HB s2/=fA; rewrite HB//.
+    + move=> s1 B HB s2/= /[!failed_or_None] fA; rewrite HB//.
     + move=> A HA B0 B HB s/=.
+      rewrite failed_and.
       case X: failed => /=.
         move=>_; rewrite HA => //.
       move=>/andP[sA fB].
@@ -166,21 +146,14 @@ Section RunP.
     move=><-; clear r.
     elim: A s1; try by move=> // s1 <-//=.
     - move=> A HA s B HB s1/=; have:= HA s1; case_step_tag X B1 => //=.
-    - move=> s B HB s1/=; have:= HB s; case_step_tag X B1 => //=.
-    - move=> A HA B0 B HB s1/=.
+    - move=> s B HB s1/= /[!failed_or_None] ; have:= HB s; case_step_tag X B1 => //=.
+    - move=> A HA B0 B HB s1/=/[!failed_and].
       have:= HA s1.
       case_step_tag X A1 => //=; only 1,2: by move=> H/H->; rewrite (step_not_solved X).
       move=> /(_ notF)->//=.
       have [[-> <-] ->]:= (step_success X); subst.
       by rewrite 2!push /= => /HB.
   Qed.
-
-  Lemma is_ko_big_or r A: is_ko (big_or r A) = false.
-  Proof. by elim: A r => //=[|[s r] rs IH] r1/=; rewrite is_ko_big_and//. Qed.
-
-  Lemma step_is_ko u p fv s1 A r:
-    step u p fv s1 A = r -> ~ (is_fl r.1.2) -> is_ko A = false.
-  Proof. by move=>*; apply/failed_is_ko/step_not_failed; eassumption. Qed.
 
   (********************************************************************)
   (* NEXT_ALT OP PROPERTIES                                           *)
@@ -191,21 +164,16 @@ Section RunP.
     move=><-; elim: A b {r} => //=.
     - move=> []//.
     - move=> A HA s B HB b; have:= HA b; case: next_alt => //=.
-      by have:= HB false; case: next_alt.
-    - move=> s B HB b; have:= HB b; case: next_alt => //=.
+      by have:= HB false; case: next_alt => //= ?; rewrite failed_or_None.
+    - by move=> s B HB b; have:= HB b; case: next_alt => //=*; rewrite failed_or_None.
     - move=> A HA l B HB b.
       case sA: success.
-        have:= HB b; case: next_alt => //=.
-          by move=> ? ->; rewrite sA success_failed.
-        by have:= HA true; case: next_alt => //=A' ->; rewrite failed_big_and andbF.
-      case: ifP => /=fA; last by rewrite sA fA.
-      by have:= HA false; case: next_alt => //= ? ->; rewrite failed_big_and andbF.
-  Qed.
-
-  Lemma next_alt_is_ko {b A r}: next_alt b A = r -> (is_ko (odflt OK r) = false)%type2.
-  Proof.
-    move=>/next_alt_failed.
-    by move=> /failed_is_ko.
+        have:= HB b; case: next_alt => [A'|]//=.
+          rewrite failed_and.
+          by move=> ->; rewrite sA success_failed.
+        by have:= HA true; case: next_alt => //= A' /[!failed_and] ->; rewrite failed_big_and andbF.
+      case: ifP => /=fA; last by rewrite failed_and sA fA.
+      by have:= HA false; case: next_alt => //= ? /[!failed_and] ->; rewrite failed_big_and andbF.
   Qed.
 
   Lemma failed_big_or u p fv s t: failed (backchain u p fv s t).2.
@@ -279,54 +247,35 @@ Section RunP.
     Qed.
   End same_structure.
 
+  Lemma get_subst_or_None s sm B: get_subst s (Or None sm B) = get_subst sm B.
+  Proof. by rewrite/get_subst/=. Qed.
+  
+  Lemma get_subst_or_Some s sm A B: get_subst s (Or (Some A) sm B) = get_subst s A.
+  Proof. by rewrite/get_subst/=. Qed.
+
+  Lemma get_subst_and s A B0 B : 
+    get_subst s (And A B0 B) = if success A then get_subst (get_subst s A) B else get_subst s A. 
+  Proof. by rewrite/get_subst/success/=/path_end push !path_endP; case: path_end => //. Qed.
+
   Lemma ges_subst_cutl {s A} : 
     success A -> get_subst s (cutl A) = get_subst s A.
   Proof.
-    elim: A s => //=; auto.
-    move=> A HA B0 B HB s /andP[sA sB]; rewrite sA/=success_cut sA HA// HB//.
+    elim_tree A s => //=; auto.
+      move=> /[!success_or_Some]/HA{}HA/[!get_subst_or_Some]//.
+      move=> /[!success_or_None]/HB{}HB/[!get_subst_or_None]//.
+    rewrite success_and fun_if !get_subst_and success_cut => /andP[sA sB].
+    by rewrite sA HB//HA//.
   Qed.
 
   Lemma next_alt_not_failed {A}:
-    (failed A) = false -> next_alt false A = Some A.
+    failed A = false -> next_alt false A = Some A.
   Proof.
     elim: A => //=.
     - move=> A HA s B HB fA; rewrite HA//=.
-    - move=> s B HB fB; rewrite HB//=.
-    - move=> A HA l B HB.
+    - move=> s B HB /[!failed_or_None] fB; rewrite HB//=.
+    - move=> A HA l B HB /[!failed_and].
       case fA: failed => //.
       case sA: success => //= fB; rewrite (HA, HB)//=.
-  Qed.
-
-  Lemma next_alt_not_success {A b}:
-    failed A = false ->
-      (success A) = false -> next_alt b A = Some A.
-  Proof.
-    elim: A => //=.
-    - move=> A HA s B HB fA sA; rewrite HA//.
-    - move=> s B HB fA sA; rewrite HB//.
-    - move=> A HA l B HB.
-      case fA: failed => //=.
-      case sA: success => //= fB sV.
-      rewrite HB//.
-  Qed.
-
-  Lemma next_alt_alt_None_sf {b A}:
-    next_alt b A = None -> success A \/ failed A.
-  Proof.
-    case s: success; auto.
-    case f: failed; auto.
-    rewrite next_alt_not_success//.
-  Qed.
-
-  Lemma next_alt_false_true {A b}:
-    success A = false ->
-      next_alt b A = next_alt false A.
-  Proof.
-    elim: A b => //=.
-    - move=> A HA s B HB b sA; rewrite HA//.
-    - move=> s B HB b sA; rewrite HB//.
-    - move=> A HA l B HB b.
-      by case sA: success => //=sB; rewrite HB//.
   Qed.
 
   Lemma next_alt_big_and r:
@@ -343,25 +292,6 @@ Section RunP.
   Lemma get_substS_big_and A s1:
     get_subst s1 (big_and A) = s1.
   Proof. elim: A => //. Qed.
-
-  Lemma is_ko_run u p fv s A: is_ko A -> run u p fv s A None None false fv.
-  Proof.
-    elim_tree A s => /=.
-    - by move=> _; apply: run_dead => //=.
-    - move=> /andP[kA kB].
-      have {}HA := HA s kA.
-      have {}HB := HB s kB.
-      apply: run_dead; rewrite/=.
-      by rewrite !is_ko_next_alt// !if_same.
-    - move=> kB.
-      have {}HB := HB s kB.
-      apply: run_dead; rewrite/=.
-      by rewrite !is_ko_next_alt// !if_same.
-    - move=> kA.
-      have {HB}HA := HA s kA.
-      apply: run_dead => /=.
-      by rewrite is_ko_success//=is_ko_failed//is_ko_next_alt//.
-  Qed.
 
   Lemma run_success1 u p fv A s: 
     success A -> run u p fv s A (Some (get_subst s A)) ((next_alt true A)) false fv.
